correctness/RegexCorrectness/NFA/Basic.lean
@@ -25,21 +25,21 @@ def Node.εStep (n : Node) : Set Nat :=
   | _ => ∅
 
 def charStep (nfa : NFA) (i : Nat) (c : Char) : Set Nat :=
-  if h : i < nfa.nodes.size
+  if h : i < nfa.size
     then nfa[i].charStep c
     else ∅
 
 def εStep (nfa : NFA) (i : Nat) : Set Nat :=
-  if h : i < nfa.nodes.size
+  if h : i < nfa.size
     then nfa[i].εStep
     else ∅
 
-theorem charStep_of_charStep {nfa : NFA} {i : Nat} {c : Char} {h : i < nfa.nodes.size}
+theorem charStep_of_charStep {nfa : NFA} {i : Nat} {c : Char} {h : i < nfa.size}
   {j : Nat} (mem : j ∈ nfa[i].charStep c) :
   j ∈ nfa.charStep i c := by
   simp [charStep, h, mem]
 
-theorem εStep_of_εStep {nfa : NFA} {i : Nat} {h : i < nfa.nodes.size}
+theorem εStep_of_εStep {nfa : NFA} {i : Nat} {h : i < nfa.size}
   {j : Nat} (mem : j ∈ nfa[i].εStep) :
   j ∈ nfa.εStep i := by
   simp [εStep, h, mem]
@@ -59,14 +59,14 @@ theorem lt_of_inBounds_of_εStep {node : Node} {j k : Nat}
     try cases mem <;>
     simp_all
 
-theorem lt_of_εStep {nfa : NFA} {i j : Nat} {h : i < nfa.nodes.size}
-  (wf : nfa.WellFormed) (mem : j ∈ nfa[i].εStep) : j < nfa.nodes.size := by
+theorem lt_of_εStep {nfa : NFA} {i j : Nat} {h : i < nfa.size}
+  (wf : nfa.WellFormed) (mem : j ∈ nfa[i].εStep) : j < nfa.size := by
   have inBounds := wf.inBounds ⟨i, h⟩
   simp [get_eq_nodes_get] at mem
   exact lt_of_inBounds_of_εStep inBounds mem
 
-theorem lt_of_charStep {nfa : NFA} {i j : Nat} {c : Char} {h : i < nfa.nodes.size}
-  (wf : nfa.WellFormed) (mem : j ∈ nfa[i].charStep c) : j < nfa.nodes.size := by
+theorem lt_of_charStep {nfa : NFA} {i j : Nat} {c : Char} {h : i < nfa.size}
+  (wf : nfa.WellFormed) (mem : j ∈ nfa[i].charStep c) : j < nfa.size := by
   have inBounds := wf.inBounds ⟨i, h⟩
   simp [get_eq_nodes_get] at mem
   exact lt_of_inBounds_of_charStep inBounds mem
