regex/Regex/Backtracker/Basic.lean
@@ -12,47 +12,47 @@ namespace Regex.Backtracker
 
 structure StackEntry {s : String} (σ : Strategy s) (nfa : NFA) (startPos : Pos s) where
   update : σ.Update
-  state : Fin nfa.nodes.size
+  state : Fin nfa.size
   pos : BVPos startPos
 
 def captureNextAux.pushNext {s : String} (σ : Strategy s) (nfa : NFA) (wf : nfa.WellFormed) (startPos : Pos s) (stack : List (StackEntry σ nfa startPos))
-  (update : σ.Update) (state : Fin nfa.nodes.size) (pos : BVPos startPos) :
+  (update : σ.Update) (state : Fin nfa.size) (pos : BVPos startPos) :
   List (StackEntry σ nfa startPos) :=
   match hn : nfa[state] with
   | .done => stack
   | .fail => stack
   | .epsilon state' =>
-    have isLt : state' < nfa.nodes.size := wf.inBounds' state hn
+    have isLt : state' < nfa.size := wf.inBounds' state hn
     ⟨update, ⟨state', isLt⟩, pos⟩ :: stack
   | .split state₁ state₂ =>
-    have isLt : state₁ < nfa.nodes.size ∧ state₂ < nfa.nodes.size := wf.inBounds' state hn
+    have isLt : state₁ < nfa.size ∧ state₂ < nfa.size := wf.inBounds' state hn
     ⟨update, ⟨state₁, isLt.1⟩, pos⟩ :: ⟨update, ⟨state₂, isLt.2⟩, pos⟩ :: stack
   | .save offset state' =>
-    have isLt : state' < nfa.nodes.size := wf.inBounds' state hn
+    have isLt : state' < nfa.size := wf.inBounds' state hn
     let update' := σ.write update offset pos.current
     ⟨update', ⟨state', isLt⟩, pos⟩ :: stack
   | .anchor a state' =>
-    have isLt : state' < nfa.nodes.size := wf.inBounds' state hn
+    have isLt : state' < nfa.size := wf.inBounds' state hn
     if a.test pos.current then
       ⟨update, ⟨state', isLt⟩, pos⟩ :: stack
     else
       stack
   | .char c state' =>
-    have isLt : state' < nfa.nodes.size := wf.inBounds' state hn
+    have isLt : state' < nfa.size := wf.inBounds' state hn
     if h : ∃ h : pos ≠ s.endBVPos startPos, pos.get h = c then
       ⟨update, ⟨state', isLt⟩, pos.next h.1⟩ :: stack
     else
       stack
   | .sparse cs state' =>
-    have isLt : state' < nfa.nodes.size := wf.inBounds' state hn
+    have isLt : state' < nfa.size := wf.inBounds' state hn
     if h : ∃ h : pos ≠ s.endBVPos startPos, pos.get h ∈ cs then
       ⟨update, ⟨state', isLt⟩, pos.next h.1⟩ :: stack
     else
       stack
 
 def captureNextAux {s : String} (σ : Strategy s) (nfa : NFA) (wf : nfa.WellFormed) (startPos : Pos s)
-  (visited : BitMatrix nfa.nodes.size (startPos.remainingBytes + 1)) (stack : List (StackEntry σ nfa startPos)) :
-  (Option σ.Update × BitMatrix nfa.nodes.size (startPos.remainingBytes + 1)) :=
+  (visited : BitMatrix nfa.size (startPos.remainingBytes + 1)) (stack : List (StackEntry σ nfa startPos)) :
+  (Option σ.Update × BitMatrix nfa.size (startPos.remainingBytes + 1)) :=
   match stack with
   | [] => (.none, visited)
   | ⟨update, state, pos⟩ :: stack' =>
@@ -60,19 +60,19 @@ def captureNextAux {s : String} (σ : Strategy s) (nfa : NFA) (wf : nfa.WellForm
       captureNextAux σ nfa wf startPos visited stack'
     else
       let visited' := visited.set state pos.index
-      have : nfa.nodes.size * (startPos.remainingBytes + 1) + 1 - visited'.popcount < nfa.nodes.size * (startPos.remainingBytes + 1) + 1 - visited.popcount :=
+      have : nfa.size * (startPos.remainingBytes + 1) + 1 - visited'.popcount < nfa.size * (startPos.remainingBytes + 1) + 1 - visited.popcount :=
         BitMatrix.popcount_decreasing visited state pos.index h
       if nfa[state].isDone then
         (.some update, visited')
       else
         let stack'' := captureNextAux.pushNext σ nfa wf startPos stack' update state pos
         captureNextAux σ nfa wf startPos visited' stack''
-termination_by (nfa.nodes.size * (startPos.remainingBytes + 1) + 1 - visited.popcount, stack)
+termination_by (nfa.size * (startPos.remainingBytes + 1) + 1 - visited.popcount, stack)
 
 public def captureNext {s : String} (σ : Strategy s) (nfa : NFA) (wf : nfa.WellFormed) (startPos : Pos s) : Option σ.Update :=
   go (BVPos.start startPos) (BitMatrix.zero _ _)
 where
-  go (pos : BVPos startPos) (visited : BitMatrix nfa.nodes.size (startPos.remainingBytes + 1)) : Option σ.Update :=
+  go (pos : BVPos startPos) (visited : BitMatrix nfa.size (startPos.remainingBytes + 1)) : Option σ.Update :=
   match captureNextAux σ nfa wf startPos visited [⟨σ.empty, ⟨nfa.start, wf.start_lt⟩, pos⟩] with
   | (.some update, _) => .some update
   | (.none, visited') =>
